Define increment operator with builder_op and prove lemma relating to source_op

dataplane/Examples/Increment_top.thy
@@ -1,7 +1,6 @@
 theory Increment_top
 
 imports
-  Ooo_Input_op
   Ooo_Input_top
   Dataplane.MyProduct_Instances
   Source_op
@@ -343,14 +342,5 @@ next
       done
     done
 qed
-
-record ('p, 'd, 'd1, 't) increment_state = \<open>('p, 'd, 'd1, 't) operator_state_ty\<close> + incr :: \<open>'p \<Rightarrow> 't\<close>
-
-definition increment_op where
-  \<open>increment_op ips ops os = builder_op ips ops os
-  (\<lambda>os. (\<lambda>p. case input os p of (d, t) # xs \<Rightarrow>
-    let cap = Cap (t + incr os p) p
-    in drop_cap (produce (os\<lparr>input := (input os)(p := xs)\<rparr>) cap [d]) cap)
-    |`| cfilter (\<lambda>p. input os p \<noteq> []) ops)\<close>
 
 end
