dataplane/Examples/Increment_op.thy
@@ -1,0 +1,402 @@
+theory Increment_op
+
+imports
+  Ooo_Input_op
+  Dataplane.MyProduct_Instances
+  Source_op
+begin
+
+record ('p, 'd, 'd1, 't) increment_state = \<open>('p, 'd, 'd1, 't) operator_state_ty\<close> + incr :: \<open>'p \<Rightarrow> 't\<close>
+
+definition increment_op_logic where
+  \<open>increment_op_logic ops os = cimage (\<lambda>p. case input os p of (d, t) # xs \<Rightarrow>
+    let cap = Cap (t + incr os p) p
+    in drop_cap (produce (os\<lparr>input := (input os)(p := xs)\<rparr>) cap [en1 os d]) cap)
+    (cfilter (\<lambda>p. input os p \<noteq> []) ops)\<close>
+
+definition increment_op where
+  \<open>increment_op ips ops os = builder_op ips ops os
+  (\<lambda>os. (\<lambda>p. case input os p of (d, t) # xs \<Rightarrow>
+    let cap = Cap (t + incr os p) p
+    in drop_cap (produce (os\<lparr>input := (input os)(p := xs)\<rparr>) cap [d]) cap)
+    |`| cfilter (\<lambda>p. input os p \<noteq> []) ops)\<close>
+
+abbreviation ooo_inp_op where
+  \<open>ooo_inp_op os \<equiv>
+  map_op (case_option (Inl (0 :: 2)) (\<lambda>p. Inr (0 :: 2, p))) (case_option (Inl (0 :: 2)) (\<lambda>p. Inr (0 :: 2, p)))
+  (ooo_input_op {|0 :: 1|} os)\<close>
+
+abbreviation incr_op where
+  \<open>incr_op os \<equiv>
+  map_op (case_option (Inl (1 :: 2)) (\<lambda>p. Inr (1 :: 2, p))) (case_option (Inl (1 :: 2)) (\<lambda>p. Inr (1 :: 2, p)))
+  (increment_op {|0 :: 1|} {|0|} os)\<close>
+
+abbreviation inp_incr_op where
+  \<open>inp_incr_op os1 buf os2 \<equiv>
+  map_op (case_sum id id) (case_sum id id)
+  (comp_op [Inr (0 :: 2, 0 :: 1) \<mapsto> Inr (1 :: 2, 0 :: 1)] buf (ooo_inp_op os1)
+    (incr_op os2))\<close>
+
+abbreviation inp_incr_edges where
+  \<open>inp_incr_edges \<equiv> (\<lambda>l. if l = Loc (0 :: 2) (Src (0 :: 1)) then [Loc (1 :: 2) (Trg (0 :: 1))] else [])\<close>
+
+abbreviation inp_incr_summary where
+  \<open>inp_incr_summary inc \<equiv> (\<lambda>l1 l2.
+  if l1 = Loc (0 :: 2) (Src (0 :: 1)) \<and> l2 = Loc (1 :: 2) (Trg (0 :: 1))
+  then antichain {0}
+  else if l1 = Loc 0 (Trg 0) \<and> l2 = Loc 0 (Src 0)
+  then antichain {0}
+  else if l1 = Loc 1 (Trg 0) \<and> l2 = Loc 1 (Src 0)
+  then antichain {inc}
+  else {}\<^sub>A)\<close>
+
+(* TODO relax assumptions on encoding functions. *)
+lemma ooo_input_op_increment_op_source_op:
+  \<open>summ sg = inp_incr_summary (incr os2 0) \<Longrightarrow>
+  initia os1 \<Longrightarrow> en1 os1 = id \<Longrightarrow>
+  monotone (es os1 0) (mset (ocaps os1 0)) \<Longrightarrow>
+  initia os2 \<Longrightarrow> en1 os2 = id \<Longrightarrow>
+  \<forall>x \<in> set (buf (Inr (1, 0))). is_Inr x \<Longrightarrow>
+  dataflow_op sg (inp_incr_op os1 buf os2)
+  \<approx> map_op (\<lambda>(p :: 1). (1, p)) (\<lambda>p. (1, p))
+    (source_op ((\<lambda>p. outpu os2 p @@- lmap (\<lambda>(d, t). (d, t + incr os2 p))
+      ((input os2 p @ map projr (buf (Inr (1, 0))) @ outpu os1 p) @@- lmap (\<lambda>x. case x of Data t d \<Rightarrow> (d, t)) (lfilter is_Data (es os1 p))))))\<close>
+  unfolding ooo_input_op_def ooo_input_op_logic_def increment_op_def increment_op_logic_def
+proof (coinduction arbitrary: sg os1 buf os2 rule: wbisim_coinduct_upto'')
+  case SIM1
+  then show ?case
+    apply (auto 0 0 elim!: step_dataflow_op_elim step_map_op_elim step_comp_op_elim step_builder_op_elim split: if_splits event.splits llist.splits option.splits)
+    subgoal
+      apply (intro exI conjI)
+       apply (rule step_wstep)
+       apply (rule step_map_op)
+        apply (rule step_source_op_Out_intro)
+          apply (simp_all add: defaults_num1_def)
+      apply (rule wbc_base)
+      apply (intro exI conjI)
+              apply (rule refl)
+             apply (auto intro!: arg_cong[where f=\<open>map_op _ _\<close>] arg_cong[where f=source_op] simp add: fun_eq_iff)
+      done
+    subgoal
+      apply (intro exI conjI)
+       apply (rule rtranclp.intros(1))
+      apply (rule wbc_base)
+      apply (intro exI)
+      apply auto
+      done
+    subgoal
+      using BHD_def is_Inl.simps(2) is_Inr.simps(2) list.set_sel(1) sumE
+      by (metis (no_types, opaque_lifting))
+    subgoal for d t
+      apply (intro exI conjI)
+       apply (rule rtranclp.intros(1))
+      apply (rule wbc_base)
+      apply (rule exI[of _ sg])
+      apply (rule exI[of _ os1])
+      apply (rule exI[of _ \<open>BTL (Inr (1, 0)) buf\<close>])
+      apply (rule exI[of _ \<open>consumes os2 0 t d\<close>])
+      apply (auto intro!: arg_cong[where f=\<open>map_op _ _ \<close>] arg_cong[where f=source_op] arg_cong[where f=\<open>lshift _\<close>] arg_cong[where f=\<open>lmap _\<close>] arg_cong[where f=\<open>\<lambda>x. lshift x _\<close>] simp add: produce_def BTL_def map_tl in_set_tlD fun_eq_iff)
+      using hd_Cons_tl hd_map BHD_def list.inj_map_strong list.sel(2) list.simps(14) map_tl memb_imp_not_empty not_Cons_self sum.sel(2)
+      apply (smt (verit, best))
+      done
+    subgoal
+      apply (intro exI conjI)
+       apply (rule rtranclp.intros(1))
+      apply (rule wbc_base)
+      apply (intro exI)
+      apply (auto elim: monotone.cases simp add: list.map_ident_strong)
+      done
+    subgoal
+      apply (intro exI conjI)
+       apply (rule rtranclp.intros(1))
+      apply (rule wbc_base)
+      apply (intro exI)
+      apply (auto elim: monotone.cases simp add: produce_def simp flip: snoc_shift)
+      done
+    subgoal
+      apply (intro exI conjI)
+       apply (rule rtranclp.intros(1))
+      apply (rule wbc_base)
+      apply (intro exI)
+      apply (auto elim: monotone.cases)
+      done
+    subgoal
+      apply (intro exI conjI)
+       apply (rule rtranclp.intros(1))
+      apply (rule wbc_base)
+      apply (intro exI)
+      apply (auto elim: monotone.cases)
+      done
+    subgoal
+      apply (intro exI conjI)
+       apply (rule rtranclp.intros(1))
+      apply (rule wbc_base)
+      apply (intro exI conjI)
+              apply (rule refl)
+             apply (auto simp add: produce_def fun_eq_iff split: list.splits)
+      done
+    subgoal
+      apply (intro exI conjI)
+       apply (rule rtranclp.intros(1))
+      apply (rule wbc_base)
+      apply (intro exI conjI)
+              apply (rule refl)
+             apply (auto simp add: fun_eq_iff)
+      done
+    subgoal
+      apply (intro exI conjI)
+       apply (rule rtranclp.intros(1))
+      apply (rule wbc_base)
+      apply (intro exI conjI)
+              apply (rule refl)
+             apply simp_all
+      done
+    subgoal
+      apply (intro exI conjI[rotated, OF wbc_base])
+       apply auto
+      done
+    subgoal
+      apply (intro exI conjI[rotated, OF wbc_base])
+       apply (auto simp add: fun_eq_iff)
+      done
+    done
+next
+  case SIM2
+  then show ?case
+    apply (elim step_map_op_elim step_source_op_elim conjE; simp; hypsubst_thin?; simp)
+    subgoal for x
+      apply (cases x; cases \<open>outpu os2 0\<close>; simp)
+      subgoal for d t
+        apply (cases \<open>input os2 0\<close>; simp)
+        subgoal
+          apply (cases \<open>buf (Inr (1, 1))\<close>; simp)
+          subgoal
+            apply (cases \<open>outpu os1 0\<close>; simp)
+            subgoal
+              apply (subst (asm) lmap_eq_LCons_conv)
+              apply (elim exE conjE; hypsubst_thin)
+              subgoal for x lxs
+                apply (cases x; simp)
+                subgoal for t'
+                  apply (subgoal_tac \<open>ldropWhile (Not \<circ> is_Data) (es os1 0) = LCons (Data t' d) (ltl (ldropWhile (Not \<circ> is_Data) (es os1 0)))\<close>)
+                   apply (subgoal_tac \<open>lfinite (ltakeWhile (Not \<circ> is_Data) (es os1 0))\<close>)
+                    apply (subgoal_tac \<open>initia (foldl
+                   (\<lambda>os. case_event (\<lambda>a aa. undefined) (\<lambda>t. os\<lparr>inter := operator_state.inter os @ [(1, t, - 1)], ocaps := map_entry 1 (remove_last t) (ocaps os)\<rparr>)
+                           (add_cap os 1))
+                   (os1\<lparr>es := (es os1)(1 := ltl (ldropWhile (\<lambda>x. \<not> is_Data x) (es os1 1)))\<rparr>) (list_of (ltakeWhile (\<lambda>x. \<not> is_Data x) (es os1 1))))
+               \<close>)
+                     apply (subgoal_tac \<open>en1 (foldl
+                   (\<lambda>os. case_event (\<lambda>a aa. undefined) (\<lambda>t. os\<lparr>inter := operator_state.inter os @ [(1, t, - 1)], ocaps := map_entry 1 (remove_last t) (ocaps os)\<rparr>)
+                           (add_cap os 1))
+                   (os1\<lparr>es := (es os1)(1 := ltl (ldropWhile (\<lambda>x. \<not> is_Data x) (es os1 1)))\<rparr>) (list_of (ltakeWhile (\<lambda>x. \<not> is_Data x) (es os1 1))))
+               = id\<close>)
+                  subgoal
+                    apply (intro exI conjI)
+                     apply (rule wstep_trans(1))
+                      apply (rule step_Taus_dataflow_op_Taus_intro)
+                      apply (rule rtranclp.intros(2))
+                       apply (rule rtranclp.intros(2))
+                        apply (rule rtranclp.intros(2))
+                         apply (rule step_star_map_op)
+                         apply (rule step_comp_op_L_Tau_start)
+                         apply (rule step_star_map_op)
+                         apply (rule step_Taus_ooo_input_op_Drop_Mint[where ops=\<open>{|1|}\<close>])
+                                 apply simp_all
+                         apply (unfold ooo_input_op_def ooo_input_op_logic_def)
+                         apply simp
+                        apply (rule step_map_op)
+                         apply (rule step_Tau_comp_op_L)
+                            apply (rule step_map_op)
+                             apply (rule step_builder_op_Write_Some)
+                                 apply (simp_all add: produce_def)
+                         apply (drule outpu_foldl_ooo_input_os_Drop_Mint_es_update[where xs=\<open>list_of (ltakeWhile (Not \<circ> is_Data) (es os1 0))\<close> and lxs=\<open>ltl (ldropWhile (Not \<circ> is_Data) (es os1 0))\<close>])
+                    using set_list_of ltakeWhile_all comp_apply lset_ltakeWhileD ltakeWhile_cong zero_one
+                           apply (smt (verit, best))
+                          apply (rule refl)
+                         apply simp
+                         apply (subgoal_tac \<open>(ooo_input_os_Drop_Mint 1 :: (1, 'c, 'c, 'a, 'e) input_state_scheme \<Rightarrow> ('a, 'c) event \<Rightarrow> (1, 'c, 'c, 'a, 'e) input_state_scheme)
+  = (\<lambda>os. case_event (\<lambda>a aa. undefined) (\<lambda>t. os\<lparr>inter := operator_state.inter os @ [(1, t, - 1)], ocaps := map_entry 1 (remove_last t) (ocaps os)\<rparr>) (add_cap os 1))\<close>)
+                          apply simp
+                    using event.case apply simp
+                        apply simp
+                       apply (rule step_map_op)
+                        apply (rule step_Tau_comp_op_R)
+                             apply (rule step_map_op)
+                              apply (rule step_builder_op_Read_Some)
+                                 apply auto[11]
+                      apply (rule step_map_op)
+                       apply (rule step_comp_op_R_Tau)
+                         apply (rule step_map_op)
+                          apply (rule step_builder_op_Silent)
+                             apply auto[8]
+                     apply (rule step_Out_dataflow_op_Out_Inr_intro)
+                     apply (rule step_map_op)
+                      apply (rule step_comp_op_R_Out)
+                        apply (rule step_map_op)
+                         apply (rule step_builder_op_Write_Some)
+                             apply (simp_all add: produce_def)
+                     apply simp
+                    apply (rule wbc_base)
+                    apply (subgoal_tac \<open>es (foldl
+             (\<lambda>os. case_event (\<lambda>a aa. undefined) (\<lambda>t. os\<lparr>inter := operator_state.inter os @ [(1, t, - 1)], ocaps := map_entry 1 (remove_last t) (ocaps os)\<rparr>) (add_cap os 1))
+             (os1\<lparr>es := (es os1)(1 := ltl (ldropWhile (\<lambda>x. \<not> is_Data x) (es os1 1)))\<rparr>) (list_of (ltakeWhile (\<lambda>x. \<not> is_Data x) (es os1 1))))
+         1 = ltl (ldropWhile (\<lambda>x. \<not> is_Data x) (es os1 1))\<close>)
+                     apply (intro exI conjI)
+                             apply (rule refl)
+                            apply (auto intro!: arg_cong[where f=\<open>map_op _ _\<close>] arg_cong[where f=source_op] arg_cong[where f=\<open>lmap _\<close>] simp add: fun_eq_iff)
+                    using ltl_lfilter ext comp_apply ltl_lmap ltl_simps(2) apply (metis (lifting))
+                     apply (rule monotone_ooo_input_os_Drop_Mint_es_update)
+                        apply simp
+                       apply simp
+                      apply assumption
+                     apply simp
+                    apply (rule es_foldl_ooo_input_os_Drop_Mint[where os=\<open>(os1\<lparr>es := (es os1)(1 := ltl (ldropWhile (\<lambda>x. \<not> is_Data x) (es os1 1)))\<rparr>)\<close> and xs=\<open>list_of (ltakeWhile (Not \<circ> is_Data) (es os1 0))\<close>])
+                      apply simp
+                    using set_list_of ltakeWhile_all comp_apply lset_ltakeWhileD ltakeWhile_cong zero_one
+                     apply (smt (verit, best))
+                    apply simp
+                    done
+                     apply (drule en1_foldl_ooo_input_os_Drop_Mint_es_update[where p=1 and xs=\<open>list_of (ltakeWhile (Not \<circ> is_Data) (es os1 0))\<close> and lxs=\<open>ltl (ldropWhile (Not \<circ> is_Data) (es os1 1))\<close>])
+                  using set_list_of ltakeWhile_all comp_apply lset_ltakeWhileD ltakeWhile_cong zero_one
+                       apply (smt (verit, best))
+                      apply (rule refl)
+                     apply (subgoal_tac \<open>(ooo_input_os_Drop_Mint 1 :: (1, 'c, 'c, 'a, 'e) input_state_scheme \<Rightarrow> ('a, 'c) event \<Rightarrow> (1, 'c, 'c, 'a, 'e) input_state_scheme)
+  = (\<lambda>os. case_event (\<lambda>a aa. undefined) (\<lambda>t. os\<lparr>inter := operator_state.inter os @ [(1, t, - 1)], ocaps := map_entry 1 (remove_last t) (ocaps os)\<rparr>) (add_cap os 1))\<close>)
+                      apply simp
+                  using event.case apply simp
+                    apply (drule initia_foldl_ooo_input_os_Drop_Mint_es_update[where p=1 and xs=\<open>list_of (ltakeWhile (Not \<circ> is_Data) (es os1 0))\<close> and lxs=\<open>ltl (ldropWhile (Not \<circ> is_Data) (es os1 1))\<close>])
+                  using set_list_of ltakeWhile_all comp_apply lset_ltakeWhileD ltakeWhile_cong zero_one
+                      apply (smt (verit, best))
+                     apply (rule refl)
+                    apply (subgoal_tac \<open>(ooo_input_os_Drop_Mint 1 :: (1, 'c, 'c, 'a, 'e) input_state_scheme \<Rightarrow> ('a, 'c) event \<Rightarrow> (1, 'c, 'c, 'a, 'e) input_state_scheme)
+  = (\<lambda>os. case_event (\<lambda>a aa. undefined) (\<lambda>t. os\<lparr>inter := operator_state.inter os @ [(1, t, - 1)], ocaps := map_entry 1 (remove_last t) (ocaps os)\<rparr>) (add_cap os 1))\<close>)
+                     apply simp
+                  using event.case apply simp
+                  using lfinite_ltakeWhile apply fastforce
+                  using lfilter_eq_LCons event.case_eq_if event.collapse(1) lfilter_eq_LConsD lmap_eq_LCons_conv
+                    ltl_simps(2) prod.sel(1,2) zero_one
+                  apply (smt (verit, ccfv_threshold))
+                  done
+                done
+              done
+            subgoal for x'
+              apply (erule conjE)
+              apply (cases x'; simp)
+              subgoal
+                apply (intro exI conjI)
+                 apply (rule wstep_trans(1))
+                  apply (rule rtranclp.intros(2))
+                   apply (rule rtranclp.intros(2))
+                    apply (rule rtranclp.intros(2))
+                     apply (rule rtranclp.intros(1))
+                    apply (rule step_Tau_dataflow_op_Tau_intro)
+                    apply (rule step_map_op)
+                     apply (rule step_Tau_comp_op_L)
+                        apply (rule step_map_op)
+                         apply (rule step_builder_op_Write_Some)
+                             apply auto[10]
+                   apply (rule step_Tau_dataflow_op_Tau_intro)
+                   apply (rule step_map_op)
+                    apply (rule step_Tau_comp_op_R)
+                         apply (rule step_map_op)
+                          apply (rule step_builder_op_Read_Some)
+                             apply auto[11]
+                  apply (rule step_Tau_dataflow_op_Tau_intro)
+                  apply (rule step_map_op)
+                   apply (rule step_comp_op_R_Tau)
+                     apply (rule step_map_op)
+                      apply (rule step_builder_op_Silent)
+                         apply auto[8]
+                 apply (rule step_Out_dataflow_op_Out_Inr_intro)
+                 apply (rule step_map_op)
+                  apply (rule step_comp_op_R_Out)
+                    apply (rule step_map_op)
+                     apply (rule step_builder_op_Write_Some)
+                         apply (simp_all add: produce_def)
+                 apply simp
+                apply (rule wbc_base)
+                apply (intro exI conjI)
+                        apply (rule refl)
+                       apply (auto intro!: arg_cong[where f=\<open>map_op _ _\<close>] arg_cong[where f=source_op] simp add: fun_eq_iff)
+                done
+              done
+            done
+          subgoal for x'
+            apply (cases x'; simp)
+            subgoal for x'
+              apply (cases x'; simp)
+              subgoal
+                apply (intro exI conjI)
+                 apply (rule wstep_trans(1))
+                  apply (rule rtranclp.intros(2))
+                   apply (rule rtranclp.intros(2))
+                    apply (rule rtranclp.intros(1))
+                   apply (rule step_Tau_dataflow_op_Tau_intro)
+                   apply (rule step_map_op)
+                    apply (rule step_Tau_comp_op_R)
+                         apply (rule step_map_op)
+                          apply (rule step_builder_op_Read_Some)
+                             apply (auto simp add: BHD_def)[11]
+                  apply (rule step_Tau_dataflow_op_Tau_intro)
+                  apply (rule step_map_op)
+                   apply (rule step_comp_op_R_Tau)
+                     apply (rule step_map_op)
+                      apply (rule step_builder_op_Silent)
+                         apply auto[8]
+                 apply (rule step_Out_dataflow_op_Out_Inr_intro)
+                 apply (rule step_map_op)
+                  apply (rule step_comp_op_R_Out)
+                    apply (rule step_map_op)
+                     apply (rule step_builder_op_Write_Some)
+                         apply (simp_all add: produce_def)
+                 apply simp
+                apply (rule wbc_base)
+                apply (intro exI conjI)
+                        apply (rule refl)
+                       apply (auto intro!: arg_cong[where f=\<open>map_op _ _\<close>] arg_cong[where f=source_op] simp add: fun_eq_iff BTL_def)
+                done
+              done
+            done
+          done
+        subgoal
+          apply (intro exI conjI)
+           apply (rule wstep_trans_base(1))
+            apply (rule step_Tau_dataflow_op_Tau_intro)
+            apply (rule step_map_op)
+             apply (rule step_comp_op_R_Tau)
+               apply (rule step_map_op)
+                apply (rule step_builder_op_Silent)
+                   apply auto[8]
+           apply (rule step_Out_dataflow_op_Out_Inr_intro)
+           apply (rule step_map_op)
+            apply (rule step_comp_op_R_Out)
+              apply (rule step_map_op)
+               apply (rule step_builder_op_Write_Some)
+                   apply (simp_all add: produce_def split: prod.splits)
+          apply simp
+          apply (rule wbc_base)
+          apply (intro exI conjI)
+                  apply (rule refl)
+                 apply (auto intro!: arg_cong[where f=\<open>map_op _ _\<close>] arg_cong[where f=source_op] simp add: fun_eq_iff)
+          done
+        done
+      subgoal
+        apply (intro exI conjI)
+         apply (rule step_wstep)
+         apply (rule step_Out_dataflow_op_Out_Inr_intro)
+         apply (rule step_map_op)
+          apply (rule step_comp_op_R_Out)
+            apply (rule step_map_op)
+             apply (rule step_builder_op_Write_Some)
+                 apply simp_all
+         apply simp
+        apply (rule wbc_base)
+        apply (intro exI conjI)
+                apply (rule refl)
+               apply (auto intro!: arg_cong[where f=\<open>map_op _ _\<close>] arg_cong[where f=source_op] simp add: fun_eq_iff)
+        done
+      done
+    done
+qed
+
+end
